venom/passes/fmp_lowering/proofs/dretDesugarProofsScript.sml
@@ -1,0 +1,86 @@
+(* Structural proofs for target-checked DRET desugaring. *)
+Theory dretDesugarProofs
+Ancestors
+  dretDesugarDefs irSupply
+Libs
+  bossLib listTheory
+
+Definition dret_supply_extends_def:
+  dret_supply_extends old new <=>
+    (?ids. new.irs_used_inst_ids = ids ++ old.irs_used_inst_ids /\
+           ALL_DISTINCT ids /\
+           EVERY (\id. ~MEM id old.irs_used_inst_ids) ids) /\
+    (?vars. new.irs_used_vars = vars ++ old.irs_used_vars /\
+            ALL_DISTINCT vars /\
+            EVERY (\v. ~MEM v old.irs_used_vars) vars) /\
+    new.irs_used_labels = old.irs_used_labels
+End
+
+Theorem dret_supply_extends_refl:
+  dret_supply_extends s s
+Proof
+  simp[dret_supply_extends_def] >> qexistsl [`[]`,`[]`] >> simp[]
+QED
+
+Theorem all_distinct_append_fresh:
+  ALL_DISTINCT xs /\ ALL_DISTINCT ys /\ EVERY (\x. ~MEM x ys) xs ==>
+  ALL_DISTINCT (xs ++ ys)
+Proof
+  Induct_on `xs` >> simp[] >> metis_tac[]
+QED
+
+Theorem dret_supply_extends_trans:
+  dret_supply_extends s1 s2 /\ dret_supply_extends s2 s3 ==>
+  dret_supply_extends s1 s3
+Proof
+  simp[dret_supply_extends_def] >> rpt strip_tac
+  >- (qexists `ids' ++ ids` >> gvs[] >>
+      conj_tac
+      >- (irule all_distinct_append_fresh >> simp[] >> gvs[EVERY_MEM])
+      >> gvs[EVERY_MEM])
+  >> qexists `vars' ++ vars` >> gvs[] >>
+  conj_tac
+  >- (irule all_distinct_append_fresh >> simp[] >> gvs[EVERY_MEM])
+  >> gvs[EVERY_MEM]
+QED
+
+Theorem fresh_var_extends:
+  fresh_ir_var s = (v,s') ==> dret_supply_extends s s'
+Proof
+  strip_tac >> drule fresh_ir_var_contract >> strip_tac >>
+  simp[dret_supply_extends_def] >> gvs[]
+QED
+
+Theorem fresh_id_extends:
+  ir_supply_inst_ok s /\ fresh_inst_id s = (id,s') ==>
+  dret_supply_extends s s' /\ ir_supply_inst_ok s'
+Proof
+  strip_tac >> drule fresh_inst_id_contract >> disch_then drule >> strip_tac >>
+  conj_tac >- (simp[dret_supply_extends_def] >> gvs[]) >>
+  simp[]
+QED
+
+Theorem expand_dret_pairs_empty:
+  expand_dret_pairs s cursor [] =
+    SOME (DretPairExpansion [] [] cursor s)
+Proof
+  simp[expand_dret_pairs_def]
+QED
+
+Theorem expand_dret_pairs_singleton:
+  expand_dret_pairs s cursor [x] = NONE
+Proof
+  simp[expand_dret_pairs_def]
+QED
+
+Theorem expand_dret_pairs_success_fields:
+  IS_SOME (expand_dret_pairs s cursor pairs) ==>
+  ?emitted dsts final_cursor final_supply.
+    expand_dret_pairs s cursor pairs =
+      SOME (DretPairExpansion emitted dsts final_cursor final_supply)
+Proof
+  Cases_on `expand_dret_pairs s cursor pairs` >> simp[] >>
+  Cases_on `x` >> simp[]
+QED
+
+val _ = export_theory();
